module VSet.Transform.Properties where

open import VSet.Prelude
open import VSet.Data.Fin hiding (pred)

open import VSet.Function.Injection
open import VSet.Function.Iso
open import VSet.Function.Properties
open import VSet.Data.SomeFin.Base
open import VSet.Data.SomeFin.Injection
open import VSet.Data.SomeFin.Equality
open import VSet.Transform.Sub
open import VSet.Transform.Tensor
open import VSet.Transform.Split using (âŠâ†”+; âŠâ†’+; +â†’âŠ)
open import VSet.Transform.Pred

open import Cubical.Data.Nat.Properties

ğŸ˜âŠ•â‰¡id : âˆ€ {X Y : SomeFin} â†’ (f : [ X â†£ Y ]) â†’ ğŸ˜ âŠ• f â‰ˆ f
ğŸ˜âŠ•â‰¡id {X} {Y} f = record
  { p = refl
  ; q = refl
  -- Goal: (Î» i â†’ congâ‚‚ FinFun (Î» _ â†’ 0 + X) (Î» _ â†’ 0 + Y) i) [
  --   fst (ğŸ˜ âŠ• f) â‰¡ fst f ]
  ; path = cong (Î» â—‹ x â†’ fst f x) (refl {x = f})
  }

step3 : âˆ€ {X Y : SomeFin} â†’ (f : [ X â†£ Y ]) 
      â†’ (x : Fin (X + 0)) â†’ subst Fin (sym (+-zero Y)) (fst f (subst Fin (+-zero X) x)) 
      â‰¡ âŠâ†’+ (âŠ-map (fst f) (fst ğŸ˜) (+â†’âŠ x))  
step3 {suc X} {Y} f fzero =
  subst Fin (sym (+-zero Y)) (fst f (subst Fin (+-zero (suc X)) fzero)) 
    â‰¡âŸ¨ congP (Î» i â—‹ â†’ subst Fin (sym (+-zero Y)) (fst f â—‹))
    -- Goal: subst Fin (Î» i â†’ suc (+-zero X i)) fzero â‰¡ fzero
              {!!} âŸ©
  subst Fin (sym (+-zero Y)) (fst f fzero) 
    â‰¡âŸ¨ {!cong !} âŸ©
  {!!}
    â‰¡âŸ¨ {!!} âŸ©
  âŠâ†’+ (âŠ-map (fst f) (fst ğŸ˜) (+â†’âŠ fzero)) â–¯
  where
    step4 : (Î» i â†’ Fin (+-zero (suc X) i)) [ fzero â‰¡ subst Fin (+-zero (suc X)) fzero ]
    step4 = subst-filler Fin (+-zero (suc X)) fzero
step3 {suc X} f (fsuc x) = {!!}


âŠ•ğŸ˜â‰¡id : âˆ€ {X Y : SomeFin} â†’ (f : [ X â†£ Y ]) â†’ f âŠ• ğŸ˜ â‰ˆ f
âŠ•ğŸ˜â‰¡id {X} {Y} f =
  â‰ˆsym {!!}
  where
    t : [ (X + 0) â†£ (Y + 0) ]
    t = â‰ˆtransport (Î» i â†’ +-zero X (~ i)) (Î» i â†’ +-zero Y (~ i)) f 
    step1 : f â‰ˆ t
    step1 = â‰ˆcong (sym (+-zero X)) (sym (+-zero Y)) f
    open _â‰ˆ_ step1
    step2 : t â‰ˆ f âŠ• ğŸ˜
    step2 = record
      { p = refl
      ; q = refl
      ; path = funExt (Î» x â†’ 
          fst t x â‰¡âŸ¨ refl âŸ©
          subst Fin q (fst f (subst Fin (sym p) x))
            â‰¡âŸ¨ subst2-filler {!FinFun!} {!!} {!!} {!!} âŸ©
          âŠâ†’+ (âŠ-map (fst f) (fst ğŸ˜) (inl (subst Fin ((+-zero X)) x)))
            â‰¡âŸ¨ {!!} âŸ©
          âŠâ†’+ (âŠ-map (fst f) (fst ğŸ˜) (+â†’âŠ x))
            â‰¡âŸ¨ refl âŸ©
          fst (â†”toâ†£ âŠâ†”+ â†£âˆ˜â†£ â†£-map-âŠ f ğŸ˜ â†£âˆ˜â†£ â†”toâ†£ (flip-â†” âŠâ†”+)) x
            â‰¡âŸ¨ refl âŸ©
          fst (f âŠ• ğŸ˜) x â–¯)
      }
    
    -- -fâŠ•ğŸ˜
-- record
--   { p = +-zero X
--   ; q = +-zero Y
--   -- Goal: (Î» i â†’ congâ‚‚ FinFun (+-zero X) (+-zero Y) i) [ fst (f âŠ• ğŸ˜) â‰¡
--   --  fst f ]
--   ; path = Î» i x â†’ c2 {!!} {!!}
--   }
--   where
--     f' : [ X + 0 â†£ Y + 0 ]
--     f' = f âŠ• ğŸ˜
--     -- c2 : ? [ FinFun X Y â‰¡ FinFun (X + 0) (Y + 0) ]
--     c2 : (i : I) â†’ congâ‚‚ FinFun (+-zero X) (+-zero Y) i
--     c2 i x = y
--       where
--         x' : Fin X
--         x' = transport (Î» j â†’ Fin (+-zero X (i âˆ¨ j))) x
--         y' : Fin Y
--         y' = fst f x'
--         y : Fin (+-zero Y i)
--         y = transportâ» (Î» j â†’ Fin (+-zero Y (i âˆ¨ j))) y'
      
    
-- ğŸ˜âŠ•â‰ˆid {X} {Y} f x = 
--   fst (ğŸ˜ âŠ• f) x â‰¡âŸ¨ refl âŸ©
--   fst (â†”toâ†£ âŠâ†”+ â†£âˆ˜â†£ â†£-map-âŠ ğŸ˜ f â†£âˆ˜â†£ â†”toâ†£ (flip-â†” âŠâ†”+)) x â‰¡âŸ¨ refl âŸ©
--   (fst (â†”toâ†£ âŠâ†”+) âˆ˜ fst (â†£-map-âŠ ğŸ˜ f) âˆ˜ fst (â†”toâ†£ (flip-â†” âŠâ†”+))) x â‰¡âŸ¨ refl âŸ©
--   âŠâ†’+ (âŠ-map (Î» ()) (fst f) (+â†’âŠ x)) â‰¡âŸ¨ refl âŸ©
--   âŠâ†’+ (inr (fst f x)) â‰¡âŸ¨ refl âŸ©
--   fst f x â–¯

{-
finPath : (n : â„•) â†’ Fin n â‰¡ Fin (n + 0)
finPath n = cong Fin (sym (+-zero n))

x1 : Fin 1
x1 = fzero 
refl1 : x1 â‰¡ x1
refl1 = refl
x2 : Fin (1 + 0)
x2 = fzero

q = subst Fin (+-zero 1) x2

r : Fin 1 â‰¡ Fin (1 + 0)
r = subst (Î» â—‹ â†’ Fin â—‹ â‰¡ Fin (â—‹ + 0)) (+-zero 1) (cong Fin (sym (+-zero 1)))

w : âˆ€ {m : â„•} â†’ fzero {n = m} â‰¡ subst Fin (cong suc (+-zero m)) (fzero {n = m + 0})
w {m} = transport (cong (Î» â—‹ â†’ fzero {n = m} â‰¡ Fin {!suc â—‹!} ) {!!}) {!!} {!!}

foo : âˆ€ (n m : â„•) â†’ (f : Fin n â†’ Fin m) â†’ (g : Fin (n + 0) â†’ Fin (m + 0)) â†’ Type
foo n m f g = PathP (Î» i â†’ (x : Fin n) â†’ (Fin (m + 0)))
  (g âˆ˜ subst Fin (sym (+-zero n))) 
  (subst Fin (sym (+-zero m)) âˆ˜ f)



-- âŠ•ğŸ˜â‰ˆid : âˆ€ {X Y : SomeFin} â†’ (f : [ X â†£ Y ]) â†’ f âŠ• ğŸ˜ â‰ˆ f
-- âŠ•ğŸ˜â‰ˆid {X} {Y} f x =  ?
--   -- fst (f âŠ• ğŸ˜) x â‰¡âŸ¨ refl âŸ©
  -- fst (â†”toâ†£ âŠâ†”+ â†£âˆ˜â†£ â†£-map-âŠ f ğŸ˜ â†£âˆ˜â†£ â†”toâ†£ (flip-â†” âŠâ†”+)) x â‰¡âŸ¨ refl âŸ©
  -- (fst (â†”toâ†£ âŠâ†”+) âˆ˜ fst (â†£-map-âŠ f ğŸ˜) âˆ˜ fst (â†”toâ†£ (flip-â†” âŠâ†”+))) x â‰¡âŸ¨ refl âŸ©
  -- âŠâ†’+ (âŠ-map (Î» ()) (fst f) {!+â†’âŠ x!}) â‰¡âŸ¨ refl âŸ©
  -- âŠâ†’+ (inl (fst f x)) â‰¡âŸ¨ refl âŸ©
  -- fst f x â–¯

lemma1-3 : âˆ€ (X Y A : SomeFin) â†’ (f : [ X â†£ Y ])
         â†’ sub A (ladd A f) â‰ˆ f
lemma1-3 X Y zero f = {!!}
lemma1-3 X Y (suc A) f =
  {!!}

lemma1-4 : âˆ€ (X Y A B : SomeFin) â†’ (f : [ A + X â†£ A + Y ])
         â†’ radd B (sub A f) â‰ˆ sub A {!add B f!} 

-- -}
-- -}
-- -}
-- -}
-- -}
